VisualProof/Rule/WirePrimitive.lean
@@ -2,6 +2,7 @@ import VisualProof.Rule.WirePrimitive.Partition
 import VisualProof.Rule.WirePrimitive.ContentWitnesses
 import VisualProof.Rule.WirePrimitive.Content
 import VisualProof.Rule.WirePrimitive.Arguments
+import VisualProof.Rule.WirePrimitive.ArgumentsDropTransport
 import VisualProof.Rule.WirePrimitive.Leaves
 import VisualProof.Rule.WirePrimitive.Program
 
